coq_session_new/proc_csubst.v
@@ -1,0 +1,24 @@
+From mathcomp Require Import ssreflect ssrbool eqtype ssrnat seq zify.
+From Coq Require Import ssrfun Classical Utf8.
+Require Export AutosubstSsr ARS tllc_csubst dyn_csubst proc_cren.
+
+Set Implicit Arguments.
+Unset Strict Implicit.
+Unset Printing Implicit Defensive.
+
+Lemma proc_csubstitution Θ2 Θ1 p σ :
+  Θ2 ⊢ p -> Θ1 ⊩ σ ⫣ Θ2 -> Θ1 ⊢ proc_csubst p σ. 
+Proof with eauto.
+  move=>ty. elim: ty Θ1 σ=>{Θ2 p}.
+  { move=>Θ m tym Θ1 σ agr. constructor.
+    apply: dyn_csubstitution... }
+  { move=>Θ1 Θ2 Θ p q mrg typ ihp tyq ihq Θ0 σ agr. simpl.
+    have[Θa[Θb[mrgx[agr1 agr2]]]]:=dyn_agree_csubst_merge agr mrg.
+    have{}ihp:=ihp _ _ agr1.
+    have{}ihq:=ihq _ _ agr2.
+    econstructor... }
+  { move=>Θ p r1 r2 A xor typ ihp Θ1 σ agr. simpl.
+    have wf:=proc_type_wf typ. inv wf. inv H1.
+    econstructor... apply: ihp.
+    repeat constructor... }
+Qed.
