coq_session_new/tllc_csubst.v
@@ -1,0 +1,33 @@
+From mathcomp Require Import ssreflect ssrbool eqtype ssrnat seq.
+From Coq Require Import ssrfun Classical Utf8.
+Require Export AutosubstSsr ARS tll_csubst tllc_cren.
+
+Set Implicit Arguments.
+Unset Strict Implicit.
+Unset Printing Implicit Defensive.
+
+Fixpoint proc_csubst (p : proc) (σ : cvar -> term) :=
+  match p with
+  | Exp m => Exp (term_csubst m σ)
+  | Par p q => Par (proc_csubst p σ) (proc_csubst q σ)
+  | Nu p => Nu (proc_csubst p (upp (upp σ)))
+  end.
+
+Lemma proc_csubst_cids p : proc_csubst p cids = p. 
+Proof with eauto.
+  elim: p=>//=...
+  { move=>m. rewrite term_csubst_cids... }
+  { move=>p ihp q ihq. autorew... }
+  { move=>p e. rewrite! upp_cids. rewrite e... }
+Qed.
+
+Lemma proc_csubst_comp p σ1 σ2 :
+  proc_csubst (proc_csubst p σ1) σ2 = proc_csubst p (σ1 >>> term_csubst^~ σ2).
+Proof.
+  elim: p σ1 σ2=>//=.
+  { move=>m σ1 σ2. by rewrite term_csubst_comp. }
+  { move=>p ihp q ihq σ1 σ2. by autorew. }
+  { move=>p ihp σ1 σ2. f_equal.
+    rewrite ihp. f_equal.
+    apply: (term_uppn_comp σ1 σ2 2). }
+Qed.
